by-hand typechecking of testChoose10, and adjusting the definition of the type system accordingly: - adding some subtyping rules - handling type inference in data type declaration - adding rules for valuing in behaviors

types/coq/Utils.v
@@ -17,3 +17,72 @@ Notation "'values' e 'for' x 'of' f 'are' 'distinct'" :=
 Notation "'for' 'each' e f 'of' l m , p" :=
   (List.Forall2 (fun e f => p) l m)
     (at level 200, e ident, f ident, right associativity, l at level 1, m at level 1).
+
+(**
+ * Some utility functions
+
+ *)
+
+Import ListNotations.
+
+Section Decs.
+  Variable A: Type.
+  Variable A_dec: forall (x y: A), {x = y} + {x <> y}.
+
+  Definition Some_dec (l: option A) (r: option A): {l = r} + {l <> r}.
+  Proof.
+    refine (match l with
+              | Some ll => _
+              | None => _
+            end).
+    - refine (match r with
+                | Some rr => _
+                | None => _
+              end).
+      + refine (match A_dec ll rr with
+                  | left H => _
+                  | right H => _
+                end).
+        * left. f_equal. exact H.
+        * right. intro N. injection N. exact H.
+      + right. discriminate.
+    - refine (match r with
+                | Some _ => _
+                | None => _
+              end).
+      + right. discriminate.
+      + left. reflexivity.
+  Defined.
+
+  Fixpoint NoDup_dec (l: list A) {struct l}: {NoDup l} + {~ NoDup l}.
+  Proof.
+    refine (match l with
+              | [] => _
+              | hd :: tl => _
+            end).
+    - left. apply NoDup_nil.
+    - refine (match (in_dec A_dec hd tl) with
+                | left H => _
+                | right H => _
+              end).
+      + right. intro N. inversion N. contradiction.
+      + refine (match (NoDup_dec tl) with
+                  | left R => _
+                  | right R => _
+                end).
+        * left. exact (NoDup_cons _ H R).
+        * right. intro N. inversion N. contradiction.
+  Defined.
+End Decs.
+
+Ltac decide_nodup dec :=
+  match goal with
+    | |- NoDup ?l =>
+      let x := fresh "x" in
+      let E := fresh "E" in
+      remember (NoDup_dec _ dec l) as x eqn:E;
+        vm_compute in E;
+        match goal with
+          | H: (x = left ?P) |- _ => exact P
+        end
+  end.
