types/coq/tests/testDone_proof.v
@@ -4,6 +4,8 @@ Require Import testDone.
 Import List.
 Import AST.
 Import ListNotations.
+Import Utils.
+Import String.
 
 Local Open Scope string_scope.
 Local Open Scope list_scope.
@@ -18,17 +20,15 @@ Proof.
   apply type_EntityBlock_system with "test"; split.
   - apply type_SystemDecl; split.
     + apply Forall_nil.
-    + apply type_SystemDecl_datatype with "type1"; repeat split.
+    + apply type_SystemDecl_datatype_None with BooleanType; repeat split.
       * apply type_DataTypeDecl_None.
       * { apply type_SystemDecl_gate with "gate1"; repeat split.
-          - admit.
-          - simpl. apply NoDup_cons.
-            + auto.
-            + apply NoDup_nil.
+          - admit. (* TODO protocol *)
+          - simpl. decide_nodup (Some_dec _ string_dec).
           - apply Forall_cons.
             + apply type_Connection.
-              * { apply type_NamedType with (DataTypeDecl (Some "type1") None []).
-                  - admit. }
+              apply type_NamedType with (DataTypeDecl (Some "type1") (Some BooleanType) []).
+              vm_compute. reflexivity.
             + apply Forall_nil.
           - apply type_SystemDecl_None.
             + apply type_BehaviorDecl.
